back to work

code/experimental/P256/Hacl.Impl.SolinasReduction.fst
@@ -2,6 +2,7 @@ module Hacl.Impl.SolinasReduction
 
 open FStar.HyperStack.All
 open FStar.HyperStack
+module ST = FStar.HyperStack.ST
 
 open Lib.IntTypes 
 open FStar.Math.Lemmas
@@ -11,6 +12,9 @@ open Lib.Buffer
 open Hacl.Spec.P256.SolinasReduction
 open Hacl.Impl.Gen
 open Hacl.Spec.P256.Core
+open Hacl.Spec.P256.Definitions
+open FStar.Mul
+
 
 module Seq = Lib.Sequence
 
@@ -22,210 +26,343 @@ val load_buffer: a0: uint64 -> a1: uint64 -> a2: uint64 -> a3: uint64 -> o: lbuf
     (requires fun h -> live h o)
     (ensures fun h0 _ h1 -> modifies1 o h0 h1 /\ 
       (
-	let o = as_seq h1 o in  Seq.index o 0 == a0 /\ Seq.index o 1 == a1 /\ Seq.index o 2 == a2 /\ Seq.index o 3 == a3
+	let o = as_seq h1 o in 
+	felem_seq_as_nat o = uint_v a0 + uint_v a1 * pow2 64 + uint_v a2 * pow2 128 + uint_v a3 * pow2 192
       )
 )
+
 let load_buffer a0 a1 a2 a3 o = 
+  assert_norm (pow2 64 * pow2 64 = pow2 128);
+  assert_norm (pow2 64 * pow2 64 * pow2 64 = pow2 192);
   upd o (size 0) a0;
   upd o (size 1) a1;
   upd o (size 2) a2;
   upd o (size 3) a3
 
 
-val upl_zer_buffer: a0: uint32 -> a1: uint32 -> a2: uint32 -> a3: uint32 -> a4: uint32 -> 
-  a5: uint32 -> a6: uint32 -> a7: uint32
+val upl_zer_buffer: c0: uint32 -> c1: uint32 -> c2: uint32 -> c3: uint32 -> c4: uint32 -> 
+  c5: uint32 -> c6: uint32 -> c7: uint32
+  -> temp: lbuffer uint64 (size 4) 
   -> o: lbuffer uint64 (size 4) -> 
   Stack unit
-    (requires fun h -> live h o)
-    (ensures fun h0 _ h1 -> modifies1 o h0 h1)
+    (requires fun h -> live h o /\ live h temp /\ disjoint o temp)
+    (ensures fun h0 _ h1 -> modifies2 o temp h0 h1 /\ 
+      (
+	let o = as_seq h1 o in 
+	felem_seq_as_nat o == 
+	  (uint_v c0 + uint_v c1 * pow2 (1 * 32) + uint_v c2 * pow2 (2 * 32) + uint_v c3 * pow2 (3 * 32) + 
+	  uint_v c4 * pow2 (4 * 32) + uint_v c5 * pow2 (5 * 32) + uint_v  c6 * pow2 (6 * 32) + 
+	  uint_v c7 * pow2 (7 * 32)) % prime
+      )
+   )
 
-let upl_zer_buffer c0 c1 c2 c3 c4 c5 c6 c7 o = 
+let upl_zer_buffer c0 c1 c2 c3 c4 c5 c6 c7 temp o = 
     let b0 = store_high_low_u c1 c0 in 
     let b1 = store_high_low_u c3 c2 in 
     let b2 = store_high_low_u c5 c4 in 
     let b3 = store_high_low_u c7 c6 in 
-    load_buffer b0 b1 b2 b3 o;
-    reduction_prime_2prime_impl o o
+      assert_norm (pow2 (3 * 32) * pow2 (2 * 32) = pow2 (5 * 32));
+      assert_norm (pow2 (4 * 32) * pow2 (2 * 32) = pow2 (6 * 32));
+      assert_norm (pow2 (5 * 32) * pow2 (2 * 32) = pow2 (7 * 32));
+    load_buffer b0 b1 b2 b3 temp;
+    reduction_prime_2prime_impl temp o
 
 
-val upl_fir_buffer: a0: uint32 -> a1: uint32 -> a2: uint32 -> a3: uint32 -> a4: uint32
+val upl_fir_buffer: c11: uint32 -> c12: uint32 -> c13: uint32 -> c14: uint32 -> c15: uint32
+  -> temp: lbuffer uint64 (size 4) 
   -> o: lbuffer uint64 (size 4) -> 
   Stack unit
-    (requires fun h -> True)
-    (ensures fun h0 _ h1 -> True)
+    (requires fun h -> live h o /\ live h temp /\ disjoint o temp)
+    (ensures fun h0 _ h1 -> modifies2 o temp h0 h1 /\
+      (
+	let o = as_seq h1 o in 
+	felem_seq_as_nat o == 
+	  (uint_v c11 * pow2 (3 * 32) + uint_v c12 * pow2 (4 * 32) + uint_v c13 * pow2 (5 * 32) + 
+	   uint_v c14 * pow2 (6 * 32) + uint_v c15 * pow2 (7 * 32)) % prime
+      )
+   )
 
-let upl_fir_buffer c11 c12 c13 c14 c15 o = 
+
+let upl_fir_buffer c11 c12 c13 c14 c15 temp o = 
+  assert_norm (pow2 (1 * 32) * pow2 (2 * 32) = pow2 (3 * 32));
+  assert_norm (pow2 (2 * 32) * pow2 (2 * 32) = pow2 (4 * 32));
+  assert_norm (pow2 (3 * 32) * pow2 (2 * 32) = pow2 (5 * 32));
+  assert_norm (pow2 (4 * 32) * pow2 (2 * 32) = pow2 (6 * 32));
+  assert_norm (pow2 (5 * 32) * pow2 (2 * 32) = pow2 (7 * 32));
   let b0 = u64(0) in 
   let b1 = store_high_low_u c11 (u32 0) in 
   let b2 = store_high_low_u c13 c12 in 
   let b3 = store_high_low_u c15 c14 in 
-  load_buffer b0 b1 b2 b3 o;
-  reduction_prime_2prime_impl o o
+  load_buffer b0 b1 b2 b3 temp;
+  reduction_prime_2prime_impl temp o
 
 
-val upl_sec_buffer: a0: uint32 -> a1: uint32 -> a2: uint32 -> a3: uint32 
+val upl_sec_buffer: c12: uint32 -> c13: uint32 -> c14: uint32 -> c15: uint32 
   -> o: lbuffer uint64 (size 4) -> 
   Stack unit
-    (requires fun h -> True)
-    (ensures fun h0 _ h1 -> True)
+    (requires fun h -> live h o )
+    (ensures fun h0 _ h1 -> modifies1 o h0 h1 /\
+      (
+      	let o = as_seq h1 o in felem_seq_as_nat o == 
+	     (uint_v c12 * pow2 (3 * 32) + uint_v c13 * pow2 (4 * 32) + 
+        uint_v c14 * pow2 (5 * 32) + uint_v c15 * pow2 (6 * 32)) % prime
+      )
+ )
+
 
 let upl_sec_buffer c12 c13 c14 c15 o = 
+  assert_norm (pow2 (1 * 32) * pow2 (2 * 32) = pow2 (3 * 32));
+  assert_norm (pow2 (2 * 32) * pow2 (2 * 32) = pow2 (4 * 32));
+  assert_norm (pow2 (3 * 32) * pow2 (2 * 32) = pow2 (5 * 32));
+  assert_norm (pow2 (4 * 32) * pow2 (2 * 32) = pow2 (6 * 32));
     let b0 = u64 (0) in 
     let b1 = store_high_low_u c12 (u32 0) in 
     let b2 = store_high_low_u c14 c13 in 
     let b3 = store_high_low_u (u32 0) c15 in
     load_buffer b0 b1 b2 b3 o;
-    reduction_prime_2prime_impl o o
+    
+    let h1 = ST.get() in 
+    let o = as_seq h1 o in 
+    modulo_lemma (felem_seq_as_nat o) prime
 
 
-val upl_thi_buffer: a0: uint32 -> a1: uint32 -> a2: uint32 -> a3: uint32 -> a4: uint32 
+val upl_thi_buffer: c8: uint32 -> c9: uint32 -> c10: uint32 -> c14: uint32 -> c15: uint32 
+  -> temp: lbuffer uint64 (size 4) 
   -> o: lbuffer uint64 (size 4) -> 
   Stack unit
-    (requires fun h -> True)
-    (ensures fun h0 _ h1 -> True)
+ (requires fun h -> live h o /\ live h temp /\ disjoint o temp)
+    (ensures fun h0 _ h1 -> modifies2 o temp h0 h1 /\
+      (
+	let o = as_seq h1 o in felem_seq_as_nat o == 
+	  (
+      uint_v c8 + uint_v c9 * pow2 32 + uint_v c10 * pow2 (2 * 32) + 
+      uint_v c14 * pow2 (6 * 32) + uint_v c15 * pow2 (7 * 32)) % prime
+    )
+ )  
+	
 
-let upl_thi_buffer c8 c9 c10 c14 c15 o = 
+let upl_thi_buffer c8 c9 c10 c14 c15 temp o = 
+  assert_norm (pow2 (1 * 32) * pow2 (2 * 32) = pow2 (3 * 32));
+  assert_norm (pow2 (2 * 32) * pow2 (2 * 32) = pow2 (4 * 32));
+  assert_norm (pow2 (3 * 32) * pow2 (2 * 32) = pow2 (5 * 32));
+  assert_norm (pow2 (4 * 32) * pow2 (2 * 32) = pow2 (6 * 32));
+  assert_norm (pow2 (5 * 32) * pow2 (2 * 32) = pow2 (7 * 32));
    let b0 = store_high_low_u c9 c8 in 
    let b1 = store_high_low_u (u32 0) c10 in 
    let b2 = u64 0 in 
    let b3 = store_high_low_u c15 c14 in 
-   load_buffer b0 b1 b2 b3 o;
-   reduction_prime_2prime_impl o o
+   load_buffer b0 b1 b2 b3 temp;
+   reduction_prime_2prime_impl temp o
 
 
-val upl_for_buffer: a0: uint32 -> a1: uint32 -> a2: uint32 -> a3: uint32 -> a4: uint32 -> 
-  a5: uint32 -> a6: uint32 
+val upl_for_buffer: c8: uint32 -> c9: uint32 -> c10: uint32 -> c11: uint32 -> c13: uint32 -> 
+  c14: uint32 -> c15: uint32 ->
+  temp: lbuffer uint64 (size 4)
   -> o: lbuffer uint64 (size 4) -> 
   Stack unit
-    (requires fun h -> True)
-    (ensures fun h0 _ h1 -> True)
+    (requires fun h -> live h o /\ live h temp /\ disjoint o temp)
+    (ensures fun h0 _ h1 -> modifies2 o temp h0 h1 /\
+      (
+	let o = as_seq h1 o in felem_seq_as_nat o == 
+	(
+    uint_v c9 + uint_v c10 * pow2 32 + uint_v c11 * pow2 (2 * 32) + 
+    uint_v c13 * pow2 (3 * 32) + uint_v c14 * pow2 (4 * 32) + 
+    uint_v c15 * pow2 (5 * 32) + uint_v c13 * pow2 (6 * 32) + 
+    uint_v c8 * pow2 (7 * 32)) % prime
+  )
+)  
 
-let upl_for_buffer c8 c9 c10 c11 c13 c14 c15 o = 
-    let b0 = store_high_low_u c10 c9 in 
-    let b1 = store_high_low_u c13 c11 in 
-    let b2 = store_high_low_u c15 c14 in 
-    let b3 = store_high_low_u c8 c13 in 
-    load_buffer b0 b1 b2 b3 o;
-    reduction_prime_2prime_impl o o
+
+let upl_for_buffer c8 c9 c10 c11 c13 c14 c15 temp o = 
+  assert_norm (pow2 (1 * 32) * pow2 (2 * 32) = pow2 (3 * 32));
+  assert_norm (pow2 (2 * 32) * pow2 (2 * 32) = pow2 (4 * 32));
+  assert_norm (pow2 (3 * 32) * pow2 (2 * 32) = pow2 (5 * 32));
+  assert_norm (pow2 (4 * 32) * pow2 (2 * 32) = pow2 (6 * 32));
+  assert_norm (pow2 (5 * 32) * pow2 (2 * 32) = pow2 (7 * 32));
+  let b0 = store_high_low_u c10 c9 in 
+  let b1 = store_high_low_u c13 c11 in 
+  let b2 = store_high_low_u c15 c14 in 
+  let b3 = store_high_low_u c8 c13 in 
+  load_buffer b0 b1 b2 b3 temp;
+  reduction_prime_2prime_impl temp o
 
 
-val upl_fif_buffer: a0: uint32 -> a1: uint32 -> a2: uint32 -> a3: uint32 -> a4: uint32 
+val upl_fif_buffer: c8: uint32 -> c10: uint32 -> c11: uint32 -> c12: uint32 -> c13: uint32 
+  -> temp: lbuffer uint64 (size 4) 
   -> o: lbuffer uint64 (size 4) -> 
   Stack unit
-    (requires fun h -> True)
-    (ensures fun h0 _ h1 -> True)
+    (requires fun h -> live h o /\ live h temp /\ disjoint o temp)
+    (ensures fun h0 _ h1 -> modifies2 o temp h0 h1 /\
+      (
+	     let o = as_seq h1 o in 
+	     felem_seq_as_nat o == (
+        uint_v c11 + uint_v c12 * pow2 32 + uint_v c13 * pow2 (2 * 32) + 
+        uint_v c8 * pow2 (6 * 32) + uint_v c10 * pow2 (7 * 32)) % prime
+      )
+ )  
 
-let upl_fif_buffer c8 c10 c11 c12 c13 o = 
+
+let upl_fif_buffer c8 c10 c11 c12 c13 temp o = 
+  
+     assert_norm (pow2 (1 * 32) * pow2 (2 * 32) = pow2 (3 * 32));
+     assert_norm (pow2 (2 * 32) * pow2 (2 * 32) = pow2 (4 * 32));
+     assert_norm (pow2 (3 * 32) * pow2 (2 * 32) = pow2 (5 * 32));
+     assert_norm (pow2 (4 * 32) * pow2 (2 * 32) = pow2 (6 * 32));
+     assert_norm (pow2 (5 * 32) * pow2 (2 * 32) = pow2 (7 * 32));
     let b0 = store_high_low_u c12 c11 in 
     let b1 = store_high_low_u (u32 0) c13 in 
     let b2 = u64 0 in 
     let b3 = store_high_low_u c10 c8 in 
-    load_buffer b0 b1 b2 b3 o;
-    reduction_prime_2prime_impl o o
+    load_buffer b0 b1 b2 b3 temp;
+    reduction_prime_2prime_impl temp o
 
 
-val upl_six_buffer: a0: uint32 -> a1: uint32 -> a2: uint32 -> a3: uint32 -> a4: uint32 -> a5: uint32
+val upl_six_buffer: c9: uint32 -> c11: uint32 -> c12: uint32 -> c13: uint32 -> c14: uint32 -> c15: uint32
+  -> temp: lbuffer uint64 (size 4) 
   -> o: lbuffer uint64 (size 4) -> 
   Stack unit
-    (requires fun h -> True)
-    (ensures fun h0 _ h1 -> True)
+    (requires fun h -> live h o /\ live h temp /\ disjoint o temp)
+    (ensures fun h0 _ h1 -> modifies2 o temp h0 h1 /\
+      (
+	let o = as_seq h1 o in 
+	felem_seq_as_nat o == (
+    uint_v c12 + uint_v c13 * pow2 32 + uint_v c14 * pow2 (2 * 32) + uint_v c15 * pow2 (3 * 32) + 
+	  uint_v c9 * pow2 (6 * 32) + uint_v c11 * pow2 (7 * 32)) % prime
+      )
+  )  
 
-let upl_six_buffer c9  c11 c12 c13 c14 c15 o = 
+
+let upl_six_buffer c9 c11 c12 c13 c14 c15 temp o = 
+  assert_norm (pow2 (1 * 32) * pow2 (2 * 32) = pow2 (3 * 32));
+  assert_norm (pow2 (2 * 32) * pow2 (2 * 32) = pow2 (4 * 32));
+  assert_norm (pow2 (3 * 32) * pow2 (2 * 32) = pow2 (5 * 32));
+  assert_norm (pow2 (4 * 32) * pow2 (2 * 32) = pow2 (6 * 32));
+  assert_norm (pow2 (5 * 32) * pow2 (2 * 32) = pow2 (7 * 32));
     let b0 = store_high_low_u c13 c12 in 
     let b1 = store_high_low_u c15 c14 in 
     let b2 = u64 0 in 
     let b3 = store_high_low_u c11 c9 in 
-    load_buffer b0 b1 b2 b3 o;
-    reduction_prime_2prime_impl o o
+    load_buffer b0 b1 b2 b3 temp;
+    reduction_prime_2prime_impl temp o
 
 
-val upl_sev_buffer: a0: uint32 -> a1: uint32 -> a2: uint32 -> a3: uint32 -> a4: uint32 -> 
-  a5: uint32 -> a6: uint32 
+val upl_sev_buffer: c8: uint32 -> c9: uint32 -> c10: uint32 -> c12: uint32 -> c13: uint32 -> 
+  c14: uint32 -> c15: uint32 
+  -> temp: lbuffer uint64 (size 4) 
   -> o: lbuffer uint64 (size 4) -> 
   Stack unit
-    (requires fun h -> True)
-    (ensures fun h0 _ h1 -> True)
+    (requires fun h -> live h o /\ live h temp /\ disjoint o temp)
+    (ensures fun h0 _ h1 -> modifies2 o temp h0 h1 /\
+      (
+	     let o = as_seq h1 o in 
+	     felem_seq_as_nat o == (
+       uint_v c13 + uint_v c14 * pow2 32 + uint_v c15 * pow2 (2 * 32) + 
+       uint_v c8 * pow2 (3 * 32) +  uint_v c9 * pow2 (4 * 32) + 
+       uint_v c10 * pow2 (5 * 32) + uint_v c12 * pow2 (7 * 32)) % prime
+      )
+  ) 
+  
 
-let upl_sev_buffer c8 c9 c10 c12 c13 c14 c15 o = 
+let upl_sev_buffer c8 c9 c10 c12 c13 c14 c15 temp o = 
+  assert_norm (pow2 (1 * 32) * pow2 (2 * 32) = pow2 (3 * 32));
+  assert_norm (pow2 (2 * 32) * pow2 (2 * 32) = pow2 (4 * 32));
+  assert_norm (pow2 (3 * 32) * pow2 (2 * 32) = pow2 (5 * 32));
+  assert_norm (pow2 (4 * 32) * pow2 (2 * 32) = pow2 (6 * 32));
+  assert_norm (pow2 (5 * 32) * pow2 (2 * 32) = pow2 (7 * 32));
     let b0 = store_high_low_u c14 c13 in 
     let b1 = store_high_low_u c8 c15 in 
     let b2 = store_high_low_u c10 c9 in 
     let b3 = store_high_low_u c12 (u32 0) in 
-    load_buffer b0 b1 b2 b3 o;
-    reduction_prime_2prime_impl o o
+    load_buffer b0 b1 b2 b3 temp;
+    reduction_prime_2prime_impl temp o
 
 
-val upl_eig_buffer: a0: uint32 -> a1: uint32 -> a2: uint32 -> a3: uint32 -> a4: uint32 -> 
-  a5: uint32 -> a6: uint32 
+val upl_eig_buffer: c9: uint32 -> c10: uint32 -> c11: uint32 -> c12: uint32 -> c13: uint32 -> 
+  c14: uint32 -> c15: uint32 
+  -> temp: lbuffer uint64 (size 4) 
   -> o: lbuffer uint64 (size 4) -> 
   Stack unit
-    (requires fun h -> True)
-    (ensures fun h0 _ h1 -> True)
+    (requires fun h -> live h o /\ live h temp /\ disjoint o temp)
+    (ensures fun h0 _ h1 -> modifies2 o temp h0 h1 /\
+      (
+	     let o = as_seq h1 o in felem_seq_as_nat o == (
+        uint_v c14 + uint_v c15 * pow2 32 + uint_v c9 * pow2 (3 * 32) + 
+        uint_v c10 * pow2 (4 * 32) + uint_v c11 * pow2 (5 * 32) + uint_v c13 * pow2 (7 * 32)) % prime
+      )
+  ) 
+  
 
-let upl_eig_buffer c9 c10 c11 c12 c13 c14 c15 o = 
+let upl_eig_buffer c9 c10 c11 c12 c13 c14 c15 temp o = 
+  assert_norm (pow2 (1 * 32) * pow2 (2 * 32) = pow2 (3 * 32));
+  assert_norm (pow2 (2 * 32) * pow2 (2 * 32) = pow2 (4 * 32));
+  assert_norm (pow2 (3 * 32) * pow2 (2 * 32) = pow2 (5 * 32));
+  assert_norm (pow2 (4 * 32) * pow2 (2 * 32) = pow2 (6 * 32));
+  assert_norm (pow2 (5 * 32) * pow2 (2 * 32) = pow2 (7 * 32));
     let b0 = store_high_low_u c15 c14 in 
     let b1 = store_high_low_u c9 (u32 0) in 
     let b2 = store_high_low_u c11 c10 in 
     let b3 = store_high_low_u c13 (u32 0) in 
-    load_buffer b0 b1 b2 b3 o;
-    reduction_prime_2prime_impl o o
+    load_buffer b0 b1 b2 b3 temp;
+    reduction_prime_2prime_impl temp o
+
 
 val solinas_reduction_impl: i: lbuffer uint64 (size 8) -> o: lbuffer uint64 (size 4) -> 
   Stack unit
-    (requires fun h -> live h i /\ live h o)
+    (requires fun h -> live h i /\ live h o /\ disjoint i o)
     (ensures fun h0 _ h1 -> True)
 
 let solinas_reduction_impl i o = 
   push_frame();
     let tempBuffer = create (size 36) (u64 0) in 
-  let i0 = index i (size 0) in 
-  let i1 = index i (size 1) in 
-  let i2 = index i (size 2) in 
-  let i3 = index i (size 3) in 
-  let i4 = index i (size 4) in 
-  let i5 = index i (size 5) in 
-  let i6 = index i (size 6) in 
-  let i7 = index i (size 7) in 
+    let redBuffer = create (size 4) (u64 0) in 
+    let t0 = sub tempBuffer (size 0) (size 4) in
+    let t1 = sub tempBuffer (size 4) (size 4) in 
+    let t2 = sub tempBuffer (size 8) (size 4) in 
+    let t3 = sub tempBuffer (size 12) (size 4) in 
+    let t4 = sub tempBuffer (size 16) (size 4) in 
+    let t5 = sub tempBuffer (size 20) (size 4) in 
+    let t6 = sub tempBuffer (size 24) (size 4) in 
+    let t7 = sub tempBuffer (size 28) (size 4) in 
+    let t8 = sub tempBuffer (size 32) (size 4) in 
 
-  let c0 = get_low_part i0 in 
-  let c1 = get_high_part i0 in 
-  let c2 = get_low_part i1 in 
-  let c3 = get_high_part i1 in   
-  let c4 = get_low_part i2 in 
-  let c5 = get_high_part i2 in   
-  let c6 = get_low_part i3 in 
-  let c7 = get_high_part i3 in   
-  let c8 = get_low_part i4 in 
-  let c9 = get_high_part i4 in   
-  let c10 = get_low_part i5 in 
-  let c11 = get_high_part i5 in   
-  let c12 = get_low_part i6 in 
-  let c13 = get_high_part i6 in   
-  let c14 = get_low_part i7 in 
-  let c15 = get_high_part i7 in
-  
-  upl_zer_buffer c0 c1 c2 c3 c4 c5 c6 c7 tempBuffer;
-  upl_fir_buffer c8 c9 c10 c11 c12 tempBuffer;
-  upl_sec_buffer c8 c9 c10 c11 tempBuffer;
-  upl_thi_buffer c8 c9 c10 c11 c12  tempBuffer;
-  upl_for_buffer c8 c9 c10 c11 c12 c13 c14  tempBuffer;
-  upl_fif_buffer c8 c9 c10 c11 c12  tempBuffer;
-  upl_six_buffer c8 c9 c10 c11 c12 c13  tempBuffer;
-  upl_sev_buffer c8 c9 c10 c11 c12 c13 c14  tempBuffer;
-  upl_eig_buffer c8 c9 c10 c11 c12 c13 c14  tempBuffer;
+    let i0 = i.(size 0) in 
+    let i1 = i.(size 1) in 
+    let i2 = i.(size 2) in 
+    let i3 = i.(size 3) in 
+    let i4 = i.(size 4) in 
+    let i5 = i.(size 5) in 
+    let i6 = i.(size 6) in 
+    let i7 = i.(size 7) in 
 
-  let t0 = sub tempBuffer (size 0) (size 4) in 
-  let t1 = sub tempBuffer (size 4) (size 4) in 
-  let t2 = sub tempBuffer (size 8) (size 4) in 
-  let t3 = sub tempBuffer (size 12) (size 4) in   
-  let t4 = sub tempBuffer (size 16) (size 4) in   
-  let t5 = sub tempBuffer (size 20) (size 4) in   
-  let t6 = sub tempBuffer (size 24) (size 4) in   
-  let t7 = sub tempBuffer (size 28) (size 4) in 
-  let t8 = sub tempBuffer (size 32) (size 4) in 
+    let c0 = get_low_part i0 in 
+    let c1 = get_high_part i0 in 
+    let c2 = get_low_part i1 in 
+    let c3 = get_high_part i1 in   
+    let c4 = get_low_part i2 in 
+    let c5 = get_high_part i2 in   
+    let c6 = get_low_part i3 in 
+    let c7 = get_high_part i3 in   
+    let c8 = get_low_part i4 in 
+    let c9 = get_high_part i4 in   
+    let c10 = get_low_part i5 in 
+    let c11 = get_high_part i5 in   
+    let c12 = get_low_part i6 in 
+    let c13 = get_high_part i6 in   
+    let c14 = get_low_part i7 in 
+    let c15 = get_high_part i7 in
 
-  p256_double t0 o;
-  p256_double t1 o;
+  upl_zer_buffer c0 c1 c2 c3 c4 c5 c6 c7 redBuffer t0; 
+  upl_fir_buffer c11 c12 c13 c14 c15 redBuffer t1;
+  upl_sec_buffer c12 c13 c14 c15 t2;
+  upl_thi_buffer c8 c9 c10 c14 c15 redBuffer  t3;
+  upl_for_buffer c8 c9 c10 c11 c13 c14 c15 redBuffer t4;
+  upl_fif_buffer c8 c10 c11 c12 c13 redBuffer  t5;
+  upl_six_buffer c9 c11 c12 c13 c14 c15 redBuffer  t6;
+  upl_sev_buffer c8 c9 c10 c12 c13 c14 c15 redBuffer t7;
+  upl_eig_buffer c9 c10 c11 c12 c13 c14 c15 redBuffer t8;
+
+  p256_add t2 t2 t2; 
+  p256_add t1 t1 t1;
   p256_add t0 t1 o;
   p256_add t2 o o;
   p256_add t3 o o;
@@ -235,6 +372,6 @@ let solinas_reduction_impl i o =
   p256_sub o t7 o;
   p256_sub o t8 o;
  
-    pop_frame()
+    pop_frame() 
 
   
