code/experimental/P256/Hacl.Spec.P256.Definitions.fst
@@ -34,15 +34,6 @@ let p256_prime_list : x:list uint64{List.Tot.length x == 4 /\
     assert_norm(0xffffffffffffffff + 0xffffffff * pow2 64 + 0xffffffff00000001 * pow2 192 == prime);
   x
   
-noextract
-let as_nat_il (h:mem) (e:ilbuffer uint64 (size 4)) : GTot nat =
-  let open Hacl.Spec.Curve25519.Field64.Definition in 
-  let s = as_seq h e in
-  let s0 = s.[0] in
-  let s1 = s.[1] in
-  let s2 = s.[2] in
-  let s3 = s.[3] in
-  as_nat4 (s0, s1, s2, s3)
 
 
 open Hacl.Spec.Curve25519.Field64.Definition
@@ -60,7 +51,7 @@ noextract
 let point_nat = nat * nat * nat
 
 noextract
-let point_seq = Lib.Sequence.lseq uint64 12 
+let point_seq = lseq uint64 12 
 
 noextract
 let felem_seq = lseq uint64 4
@@ -78,6 +69,28 @@ let felem_seq_as_nat (a: felem_seq) : Tot nat  =
   let a2 =  Lib.Sequence.index  a 2 in 
   let a3 =  Lib.Sequence.index a 3 in 
   uint_v a0 + uint_v a1 * pow2 64 + uint_v a2 * pow2 64 * pow2 64 + uint_v a3 * pow2 64 * pow2 64 * pow2 64
+
+noextract
+let felem_seq_as_nat_8 (a: lseq uint64 8) : Tot nat = 
+  let open FStar.Mul in 
+  let a0 = Lib.Sequence.index a 0 in 
+  let a1 = Lib.Sequence.index a 1 in 
+  let a2 = Lib.Sequence.index a 2 in 
+  let a3 = Lib.Sequence.index a 3 in 
+  let a4 = Lib.Sequence.index a 4 in 
+  let a5 = Lib.Sequence.index a 5 in 
+  let a6 = Lib.Sequence.index a 6 in 
+  let a7 = Lib.Sequence.index a 7 in
+  uint_v a0 + 
+  uint_v a1 * pow2 64 + 
+  uint_v a2 * pow2 64 * pow2 64 + 
+  uint_v a3 * pow2 64 * pow2 64 * pow2 64 + 
+  uint_v a4 * pow2 64 * pow2 64 * pow2 64 * pow2 64 + 
+  uint_v a5 * pow2 64 * pow2 64 * pow2 64 * pow2 64 * pow2 64 + 
+  uint_v a6 * pow2 64 * pow2 64 * pow2 64 * pow2 64 * pow2 64 * pow2 64 + 
+  uint_v a7 * pow2 64 * pow2 64 * pow2 64 * pow2 64 * pow2 64 * pow2 64 * pow2 64
+
+
 
 
 open FStar.Mul
